backend/MachMerge.v
@@ -1,0 +1,344 @@
+Require Import Coqlib Errors.
+Require Import Integers Floats AST Linking.
+Require Import Values Memory Events Globalenvs Smallstep.
+Require Import Op Locations Mach Conventions.
+
+
+Section PRESERVATION.
+Variable return_address_offset: Mach.function -> Mach.code -> ptrofs -> Prop.
+
+Hypothesis return_address_offset_exists:
+  forall f sg ros c,
+  is_tail (Mcall sg ros :: c) (fn_code f) ->
+  exists ofs, return_address_offset f c ofs.
+Hypothesis return_address_offset_determinate:
+  forall f c ofs1 ofs2,
+    return_address_offset f c ofs1 ->
+    return_address_offset f c ofs2 ->
+    ofs1 = ofs2.
+
+Variable prog: program.
+Let ge := Genv.globalenv prog.
+
+Remark extcall_arguments_determ:
+  forall rs sp m sg args1 args2,
+  extcall_arguments rs m sp sg args1 -> extcall_arguments rs m sp sg args2 -> args1 = args2.
+Proof.
+  intros until m.
+  assert (A: forall l v1 v2,
+             extcall_arg rs m sp l v1 -> extcall_arg rs m sp l v2 -> v1 = v2).
+  { intros. inv H; inv H0. congruence.
+    destruct sp; try discriminate.
+    simpl in H1, H4.
+    apply Mem.load_result in H1.
+    apply Mem.load_result in H4. congruence. }
+  assert (B: forall p v1 v2,
+             extcall_arg_pair rs m sp p v1 -> extcall_arg_pair rs m sp p v2 -> v1 = v2).
+  { intros. inv H; inv H0.
+    eapply A; eauto.
+    f_equal; eapply A; eauto. }
+  assert (C: forall ll vl1, list_forall2 (extcall_arg_pair rs m sp) ll vl1 ->
+             forall vl2, list_forall2 (extcall_arg_pair rs m sp) ll vl2 -> vl1 = vl2).
+  {
+    induction 1; intros vl2 EA; inv EA.
+    auto.
+    f_equal; eauto. }
+  intros. eapply C; eauto.
+Qed.
+
+Remark call_arguments_determ:
+  forall rs sp m sg args1 args2,
+  call_arguments rs m sp sg args1 -> call_arguments rs m sp sg args2 -> args1 = args2.
+Proof.
+  intros until m.
+  assert (A: forall l v1 v2,
+             call_arg rs m sp l v1 -> call_arg rs m sp l v2 -> v1 = v2).
+  { intros. inv H; inv H0. congruence.
+    destruct sp; try discriminate.
+    unfold load_stack in *.
+    simpl in H1, H4.
+    apply Mem.load_result in H1.
+    apply Mem.load_result in H4. congruence. }
+  assert (B: forall p v1 v2,
+             call_arg_pair rs m sp p v1 -> call_arg_pair rs m sp p v2 -> v1 = v2).
+  { intros. inv H; inv H0.
+    eapply A; eauto.
+    f_equal; eapply A; eauto. }
+  assert (C: forall ll vl1, list_forall2 (call_arg_pair rs m sp) ll vl1 ->
+             forall vl2, list_forall2 (call_arg_pair rs m sp) ll vl2 -> vl1 = vl2).
+  {
+    induction 1; intros vl2 EA; inv EA.
+    auto.
+    f_equal; eauto. }
+  intros. eapply C; eauto.
+Qed.
+
+Lemma semantics_determinate: determinate (semantics return_address_offset prog).
+Proof.
+Ltac Equalities :=
+  match goal with
+  | [ H1: ?a = ?b, H2: ?a = ?c |- _ ] =>
+      rewrite H1 in H2; inv H2; Equalities
+  | _ => idtac
+  end.
+intros; constructor; simpl; intros.
+- (* determ *)
+  inv H; inv H0; Equalities; try discriminate.
+  + split. constructor. auto.
+  + split. constructor. auto.
+  + split. constructor. auto.
+  + split. constructor. auto.
+  + split. constructor. auto.
+  + split. constructor. auto.
+  + split. constructor. auto.
+  + split. constructor.
+    assert (ra0 = ra) by (eapply return_address_offset_determinate; eauto). subst.
+    (* assert (args0 = args) by (eapply call_arguments_determ; eauto). subst. *)
+    auto.
+  + congruence.
+  + congruence.
+  + assert (ra0 = ra) by (eapply return_address_offset_determinate; eauto). subst.
+    assert (args0 = args) by (eapply call_arguments_determ; eauto). subst.
+    destruct Mem.alloc; destruct Mem.alloc; destruct sp.
+    * destruct allc as (A & B & C), allc0 as (A' & B' & C'); subst.
+      split; auto.
+      inv EV; inv EV0; try congruence.
+      constructor. Equalities.
+      assert (vl0 = vl) by (eapply eventval_list_match_determ_2; eauto). subst.
+      eapply match_traces_call.
+    * destruct allc as (A & B & C), allc0 as (A' & B' & C'); subst.
+      split; auto.
+      inv EV; inv EV0; try congruence.
+      constructor. Equalities.
+      assert (vl0 = vl) by (eapply eventval_list_match_determ_2; eauto). subst.
+      eapply match_traces_call.
+    * destruct allc as (A & B & C), allc0 as (A' & B' & C'); subst.
+      split; auto.
+      inv EV; inv EV0; try congruence.
+      constructor. Equalities.
+      assert (vl0 = vl) by (eapply eventval_list_match_determ_2; eauto). subst.
+      eapply match_traces_call.
+    * destruct allc as (A & B & C), allc0 as (A' & B' & C'); subst.
+      split; auto.
+      inv EV; inv EV0; try congruence.
+      constructor. Equalities.
+      assert (vl0 = vl) by (eapply eventval_list_match_determ_2; eauto). subst.
+      eapply match_traces_call.
+    * destruct allc as (A & B & C), allc0 as (A' & B' & C'); subst.
+      split; auto.
+      inv EV; inv EV0; try congruence.
+      constructor. Equalities.
+      assert (vl0 = vl) by (eapply eventval_list_match_determ_2; eauto). subst.
+      eapply match_traces_call.
+    * destruct Mem.set_perm; try contradiction.
+      destruct allc as (A & B & C), allc0 as (A' & B' & C'); subst.
+      split; auto.
+      inv EV; inv EV0; try congruence.
+      constructor. Equalities.
+      assert (vl0 = vl) by (eapply eventval_list_match_determ_2; eauto). subst.
+      eapply match_traces_call.
+  + split. constructor. auto.
+  + assert (vargs0 = vargs) by (eapply eval_builtin_args_determ; eauto). subst.
+    exploit external_call_determ. eexact H2. eexact H14. intros [A B].
+    split. auto. intros. destruct B; auto. subst. auto.
+  + split. constructor. auto.
+  + split. constructor. auto.
+  + split. constructor. auto.
+  + split. constructor. auto.
+  + split. constructor. auto.
+  + split. constructor.
+    subst sp sp0. Equalities. auto.
+  + assert (args0 = args) by (eapply extcall_arguments_determ; eauto). subst.
+    exploit external_call_determ. eexact H3. eexact H13. intros [A B].
+    split. auto. intros. destruct B; auto. subst. auto.
+  + destruct sp; try contradiction.
+    destruct cp_eq_dec.
+    * subst. inv EV; inv EV0; try congruence.
+      split. constructor. auto.
+      assert (res = res0) as <- by (eapply eventval_match_determ_2; eauto).
+      split. constructor. auto.
+    * destruct Mem.set_perm; try congruence.
+      inv SET_PERM; inv SET_PERM0.
+      inv EV; inv EV0; try congruence.
+      split. constructor. auto.
+      assert (res = res0) as <- by (eapply eventval_match_determ_2; eauto).
+      split. constructor. auto.
+- (* trace length *)
+  red; intros. inv H; simpl; try lia.
+  inv EV; auto.
+  eapply external_call_trace_length; eauto.
+  eapply external_call_trace_length; eauto.
+  inv EV; auto.
+- (* initial states *)
+  inv H; inv H0. subst ge0 ge1. f_equal.
+  congruence.
+  congruence.
+- (* final no step *)
+  inv H.
+  red; intros; red; intros.
+  inv H.
+- (* final states *)
+  inv H; inv H0. congruence.
+Qed.
+
+Lemma instr_dec: forall (i i': instruction),
+    {i = i'} + {i <> i'}.
+Proof.
+  decide equality; subst; auto using mreg_eq, typ_eq, Ptrofs.eq_dec, eq_operation,
+    eq_addressing, chunk_eq, signature_eq, external_function_eq, eq_condition;
+    try now (decide equality; subst; auto using mreg_eq, ident_eq).
+  decide equality.
+  decide equality; subst;
+    auto using mreg_eq, Int.eq_dec, Int64.eq_dec,
+    Float.eq_dec, Float32.eq_dec, Ptrofs.eq_dec,
+    chunk_eq, ident_eq.
+Defined.
+
+Lemma code_dec: forall (c c': code),
+    {c = c'} + {c <> c'}.
+Proof.
+  decide equality; eauto using instr_dec.
+Qed.
+
+Lemma is_tail_dec: forall f c,
+    {is_tail c (fn_code f)} + {~ is_tail c (fn_code f)}.
+Proof.
+  intros f c.
+  generalize (fn_code f) as code. clear f.
+  induction code.
+  - destruct c.
+    + left; econstructor.
+    + right; intros A; inv A.
+  - destruct IHcode.
+    + left. constructor. assumption.
+    + destruct (code_dec c (a :: code)).
+      * subst; left; constructor.
+      * right. intros A. inv A; eauto.
+Defined.
+
+Variant mergeable: state -> Prop :=
+  | mergeable_call_int:
+    forall (s : list stackframe) (fb : block) (sp : val) (sig : signature)
+      (ros : mreg + ident) (c : code) (rs : regset) (m : mem)
+      (f : function) (f' : block) (* (ra : ptrofs) *)
+      ef,
+      find_function_ptr ge ros rs = Some f' ->
+      Genv.find_funct_ptr ge fb = Some (Internal f) ->
+      (* return_address_offset f c ra -> *)
+      is_tail (Mcall sig ros :: c) (fn_code f) ->
+      bottom = comp_of f ->
+      sig = ef_sig ef ->
+
+      Genv.find_funct_ptr ge f' = Some (External ef) ->
+      mergeable (State s fb sp (Mcall sig ros :: c) rs m)
+  | mergeable_call_cross:
+    forall (s : list stackframe) (fb : block) (sp : val)
+      (sig : signature) (ros : mreg + ident) (c : code)
+      (rs : regset) (m : mem) (f : function) (f' : block)
+      (args : list val)
+      (m_res : Mem.mem') (dra dsp : option block) ef,
+      find_function_ptr ge ros rs = Some f' ->
+      Genv.find_funct_ptr ge fb = Some (Internal f) ->
+      is_tail (Mcall sig ros :: c) (fn_code f) ->
+      (* return_address_offset f c ra -> *)
+      Genv.find_funct_ptr ge f' = Some (External ef) ->
+      Genv.allowed_call ge (comp_of f) (Vptr f' Ptrofs.zero) ->
+      comp_of f <> bottom ->
+      call_arguments (undef_regs destroyed_at_function_entry rs) m sp sig args ->
+      (Genv.type_of_call (comp_of f) bottom = Genv.CrossCompartmentCall ->
+       Forall not_ptr args) ->
+      sig = ef_sig ef ->
+      call_trace ge (comp_of f) bottom (Vptr f' Ptrofs.zero) args
+        (sig_args sig) E0 ->
+      (let (m', dummy_ra) := Mem.alloc m bottom 0 0 in
+       let (m'', dummy_sp) := Mem.alloc m' bottom 0 0 in
+       match sp with
+       | Vptr bsp _ =>
+           match Mem.set_perm m'' bsp Readable with
+           | Some m''' => m_res = m''' /\ dra = Some dummy_ra /\ dsp = Some dummy_sp
+           | None => False
+           end
+       | _ => m_res = m'' /\ dra = Some dummy_ra /\ dsp = Some dummy_sp
+       end) ->
+      mergeable (State s fb sp (Mcall sig ros :: c) rs m).
+
+Lemma mergeable_dec: forall s, {mergeable s} + {not (mergeable s)}.
+Proof.
+  intros s.
+  destruct s; try now right.
+  destruct c as [|[] ?]; try now right.
+  destruct (find_function_ptr ge s0 rs) eqn:?.
+  destruct (Genv.find_funct_ptr ge b) as [[fd | ef]|] eqn:?.
+  - right. intros A; inv A; congruence.
+  - destruct (Genv.find_funct_ptr ge f) as [[fi | ?]|] eqn:?.
+    + destruct (cp_eq_dec (comp_of fi) bottom) as [cp_f_bottom | cp_f_not_bottom].
+      * destruct (signature_eq s (ef_sig ef)).
+        -- destruct (is_tail_dec fi (Mcall s s0 :: c)).
+           ++ left. econstructor; eauto.
+           ++ right. intros A; inv A; congruence.
+        -- right. intros A; inv A; congruence.
+      * destruct (Genv.allowed_call_b ge (comp_of fi) (Vptr b Ptrofs.zero)) eqn:allowed.
+        -- eapply Genv.allowed_call_reflect in allowed.
+           destruct (get_call_arguments (undef_regs destroyed_at_function_entry rs) sp m s) as [args|] eqn:get_args.
+           ++ eapply call_arguments_equiv in get_args.
+              destruct (signature_eq s (ef_sig ef));
+                destruct (is_tail_dec fi (Mcall s s0 :: c)).
+              ** destruct (Mem.alloc m bottom 0 0) as [m' dummy_ra] eqn:alloc.
+                 destruct (Mem.alloc m' bottom 0 0) as [m'' dummy_sp] eqn:alloc'.
+                 assert (Genv.type_of_call (comp_of fi) bottom = Genv.CrossCompartmentCall -> Forall not_ptr args).
+                 { simpl. destruct flowsto_dec; try congruence.
+                   exfalso; apply n; auto with comps. }
+                 assert (call_trace ge (comp_of fi) bottom (Vptr b Ptrofs.zero) args (sig_args s) nil).
+                 { constructor. simpl. destruct flowsto_dec; try congruence.
+                   exfalso; apply n; auto with comps. }
+                 destruct sp;
+                   try now (left; eapply mergeable_call_cross; eauto; rewrite alloc, alloc'; eauto).
+                 destruct (Mem.set_perm m'' b0 Readable) as [m''' |] eqn:set.
+                 { left; eapply mergeable_call_cross; eauto.
+                   rewrite alloc, alloc', set; eauto. }
+                 { right. intros A; inv A; [congruence |].
+                   rewrite alloc, alloc', set in *; auto. }
+              ** right. intros A; inv A; congruence.
+              ** right. intros A; inv A; congruence.
+              ** right. intros A; inv A; congruence.
+           ++ right. intros A; inv A; [congruence|].
+              eapply call_arguments_equiv in H13; congruence.
+        -- right. intros A; inv A; [congruence|].
+           apply Genv.allowed_call_reflect in H11. congruence.
+    + right. intros A; inv A; congruence.
+    + right. intros A; inv A; congruence.
+  - right. intros A; inv A; congruence.
+  - right. intros A; inv A; congruence.
+Defined.
+
+Lemma mergeable_safe: forall s,
+  mergeable s -> exists s', step return_address_offset ge s E0 s' /\ not (mergeable s').
+Proof.
+  intros s ?. inv H.
+  - exploit (return_address_offset_exists f (ef_sig ef) ros c); eauto.
+    intros [? ?].
+    eexists; split; [eapply exec_Mcall_int; eauto|]. intros A; inv A.
+  - exploit (return_address_offset_exists f (ef_sig ef) ros c); eauto.
+    intros [? ?].
+    eexists; split; [eapply exec_Mcall_cross; eauto|]. intros A; inv A.
+Qed.
+
+Lemma mergeable_step_not_final: forall s s' t,
+    mergeable s ->
+    step return_address_offset ge s t s' ->
+    forall n, not (final_state s' n).
+Proof.
+  intros. intros A; inv A; inv H; inv H0.
+Qed.
+
+Theorem forward_simulation_merged:
+  forward_simulation (semantics return_address_offset prog) (mergedL (semantics return_address_offset prog) mergeable).
+Proof.
+  apply forward_simulation_merged; eauto.
+  eapply semantics_determinate.
+  eapply mergeable_dec.
+  eapply mergeable_safe.
+  eapply mergeable_step_not_final.
+Qed.
+
+End PRESERVATION.
